Add pairs as test for automation.
The only part that was difficult was plug_step_unique, which was caused
by the fact that pairs, unlike any existing terms, can either by values
or terms that can step. This meant we needed to handle some new cases,
and deal with new ways of eliminating absurd cases.

All in all, seems like a success - the only non-trivial part was caused
by an actual difference, and pretty much everything else went through
with pretty easy changes (ie, adding some cases to tactics).

It also highlighted a few cases that weren't automatic enough.

STLC.v
@@ -9,18 +9,21 @@ Ltac iauto' := try solve [intuition eauto].
 
 Inductive ty  : Set :=
 | Bool : ty
-| Fun : ty -> ty -> ty.
+| Fun : ty -> ty -> ty
+| Product : ty -> ty -> ty.
 
 Inductive exp : Set :=
 | Var : string -> exp
 | Const : bool -> exp
 | Abs : string -> ty -> exp -> exp
 | App : exp -> exp -> exp
-| If : exp -> exp -> exp -> exp.
+| If : exp -> exp -> exp -> exp
+| Pair : exp -> exp -> exp.
 
 Inductive value : exp -> Prop :=
 | VBool : forall b, value (Const b)
-| VAbs : forall x t e, value (Abs x t e).
+| VAbs : forall x t e, value (Abs x t e)
+| VPair : forall v1 v2, value v1 -> value v2 -> value (Pair v1 v2).
 
 Definition tyenv := list (string * ty).
 
@@ -65,6 +68,10 @@ Inductive has_type : tyenv -> exp -> ty -> Prop :=
                         has_type Γ e2 t ->
                         has_type Γ e3 t ->
                         has_type Γ (If e1 e2 e3) t
+| TPair : forall Γ e1 e2 t1 t2, has_type Γ e1 t1 ->
+                           has_type Γ e2 t2 ->
+                           has_type Γ (Pair e1 e2)
+                                      (Product t1 t2)
 where "Γ '|--' e" := (has_type Γ e).
 
 Hint Constructors has_type ty exp value.
@@ -74,7 +81,9 @@ Inductive context : Set :=
 | CHole : context
 | CApp1 : context -> exp -> context
 | CApp2 : exp -> context -> context
-| CIf : context -> exp -> exp -> context.
+| CIf : context -> exp -> exp -> context
+| CPair1 : context -> exp -> context
+| CPair2 : exp -> context -> context.
 
 Hint Constructors context.
 
@@ -86,7 +95,12 @@ Inductive plug : context -> exp -> exp -> Prop :=
                        value v ->
                        plug (CApp2 v C) e (App v e')
 | PIf : forall e e' C e2 e3, plug C e e' ->
-                        plug (CIf C e2 e3) e (If e' e2 e3).
+                        plug (CIf C e2 e3) e (If e' e2 e3)
+| PPair1 : forall e e' C e2, plug C e e' ->
+                        plug (CPair1 C e2) e (Pair e' e2)
+| PPair2 : forall e e' C v, plug C e e' ->
+                       value v ->
+                       plug (CPair2 v C) e (Pair v e').
 
 Hint Constructors plug.
 
@@ -101,6 +115,7 @@ Fixpoint sub (x:string) (e:exp) (e':exp) : exp :=
     | If ec e1 e2 => If (sub x ec e')
                        (sub x e1 e')
                        (sub x e2 e')
+    | Pair e1 e2 => Pair (sub x e1 e') (sub x e2 e')
     end.
 
 Notation "'[' x ':=' s ']' t" := (sub x t s) (at level 20).
@@ -153,6 +168,8 @@ Ltac plug_invert :=
         |[H : plug (CApp1 _ _) _ _ |- _ ] => invert H
         |[H : plug (CApp2 _ _) _ _ |- _ ] => invert H
         |[H : plug (CIf _ _ _) _ _ |- _ ] => invert H
+        |[H : plug (CPair1 _ _) _ _ |- _ ] => invert H
+        |[H : plug (CPair2 _ _) _ _ |- _ ] => invert H
       end.
 
 Ltac use_ih_tac :=
@@ -172,13 +189,6 @@ Ltac use_ih_tac :=
     |[IH : forall a b, _ -> ?P b ?x a |- ?P ?b ?x ?a] =>
      eapply IH
   end.
-
-Ltac use_ex_tac :=
-  match goal with
-    |[H : exists _, _ |- _] => destruct H
-    |[H : _ -> exists _, _ |- _] => destruct H
-  end; eauto.
-
 
 Lemma plug_same : forall C x e1 e2,
                     plug C x e1 ->
@@ -213,6 +223,8 @@ Proof.
   solve [exists (App x e); iauto].
   solve [exists (App e x); iauto].
   solve [exists (If x e e0); iauto].
+  solve [exists (Pair x e); iauto].
+  solve [exists (Pair e x); iauto].
 Qed.
 
 Hint Resolve plug_exists.
@@ -234,6 +246,8 @@ Proof.
    | exists (CApp1 x e2)
    | exists (CApp2 v x)
    | exists (CIf x e2 e3)
+   | exists (CPair1 x e2)
+   | exists (CPair2 v x)
   ]; intros; plug_invert; iauto.
 Qed.
 
@@ -283,7 +297,11 @@ Inductive free_in : string -> exp -> Prop :=
 | free_if2 : forall x e1 e2 e3, free_in x e2 ->
                            free_in x (If e1 e2 e3)
 | free_if3 : forall x e1 e2 e3, free_in x e3 ->
-                           free_in x (If e1 e2 e3).
+                           free_in x (If e1 e2 e3)
+| free_pair1 : forall x e1 e2, free_in x e1 ->
+                          free_in x (Pair e1 e2)
+| free_pair2 : forall x e1 e2, free_in x e2 ->
+                          free_in x (Pair e1 e2).
 
 Hint Constructors free_in.
 
@@ -307,6 +325,7 @@ Fixpoint SN (T : ty) (t : exp) : Prop :=
   (match T with
      | Bool => True
      | Fun T1 T2 => forall s, SN T1 s -> SN T2 (App t s)
+     | Product T1 T2 => True
    end).
 
 Reserved Notation "Γ '|=' Σ" (at level 40).
@@ -361,26 +380,6 @@ Qed.
 
 Hint Rewrite string_dec_ne string_dec_refl.
 
-Ltac strings' x y :=
-  destruct (string_dec x y);
-  subst;
-  eauto;
-  simpl in *;
-  eauto.
-
-
-Ltac strings :=
-  repeat (match goal with
-            |[ H : context[string_dec ?x ?y] |- _ ] =>
-             strings' x y
-            |[ H : _ |- context[string_dec ?x ?y] ] =>
-             strings' x y
-          end; subst; eauto; simpl in *);
-  intuition;
-  autorewrite with core;
-  intuition.
-
-
 Ltac string_destruct :=
   repeat (match goal with
             |[ H : context[string_dec ?x ?y] |- _ ] =>
@@ -434,12 +433,6 @@ Proof.
 Qed.
 
 Hint Resolve close_closed.
-
-Ltac string_hammer :=
-  repeat (simpl in *;
-           crush;
-          string_destruct;
-          crush).
 
 Lemma close_var : forall Σ x e, closed_env Σ ->
                            lookup Σ x = Some e ->
@@ -691,14 +684,13 @@ Lemma unique_typing : forall e Γ t t',
                         t = t'.
 Proof.
   intro e.
-  induction e; intros; iauto; inversion H; inversion H0;
-  subst; iauto.
+  induction e; intros; iauto;
+  inversion H; inversion H0; iauto;
+  try (apply f_equal); try (apply f_equal2); iauto.
 
-  (* abs *)
-  assert (EQ : t'0 = t'1). iauto. subst. iauto.
   (* app *)
   assert (EQ : (Fun t1 t) = (Fun t0 t')). iauto.
-  inversion EQ. iauto.
+  inversion EQ; iauto.
 Qed.
 
 Hint Resolve unique_typing.
@@ -713,30 +705,15 @@ Lemma preservation_plug : forall C e1 e2 e1' e2' t t',
 Proof.
   intro C.
   induction C; intros; plug_invert;
-  iauto.
+  iauto; try solve
+             [inversion H; subst;
+              econstructor;
+              iauto].
 
   (* hole *)
   assert (t = t').
   eapply unique_typing; iauto.
   subst; iauto.
-
-  (* app1 *)
-  inversion H; subst;
-  econstructor.
-  eapply IHC with (e1 := e1) (e2 := e2); iauto.
-  iauto.
-
-  (* app2 *)
-  inversion H; subst;
-  econstructor;
-  iauto.
-
-  (* if *)
-  inversion H; subst.
-  econstructor.
-  eapply IHC with (e1 := e1) (e2 := e2); iauto.
-  iauto.
-  iauto.
 Qed.
 
 Hint Resolve preservation_plug.
@@ -790,6 +767,15 @@ Ltac value_invert :=
     |[H : value _ |- _] => invert H
   end.
 
+Lemma plug_values : forall e v C, plug C e v ->
+                             value v ->
+                             value e.
+Proof.
+  intros.
+  induction H; inversion H0; iauto.
+Qed.
+
+Hint Resolve plug_values.
 
 Lemma values_dont_step : forall v e, value v -> ~step v e.
 Proof.
@@ -797,7 +783,11 @@ Proof.
   match goal with
     |[H: plug _ _ (Const _) |- _] => invert H
     |[H: plug _ _ (Abs _ _ _) |- _] => invert H
-  end; subst; step_prim_invert.
+    |[H: plug _ _ (Pair _ _) |- _] => invert H
+  end; subst; try (assert (value e1) by iauto;
+                   inversion H;
+                   subst);
+  step_prim_invert.
 Qed.
 
 Hint Resolve values_dont_step.
@@ -814,8 +804,15 @@ Hint Resolve step_prim_deterministic.
 
 Ltac smash :=
   repeat try match goal with
+               |[H: plug _ ?e ?v,
+                    H1: value ?v,
+                        H2: step_prim ?e _ |- _] =>
+                assert (value e) by (eapply plug_values;
+                                     iauto);
+                  exfalso; eapply values_dont_step; iauto
                |[H : App _ _ = App _ _ |- _] => invert H
                |[H : If _ _ _ = If _ _ _ |- _] => invert H
+               |[H : Pair _ _ = Pair _ _ |- _] => invert H
                |[H : plug _ _ _ |- _] => invert H; []
                |[H : plug _ _ ?v, H1 : value ?v |- _] => invert H
                |[H : step_prim _ _ |- _] => invert H
@@ -823,6 +820,10 @@ Ltac smash :=
                |[H : value (If _ _ _) |- _] => invert H
                |[H : If _ _ _ = App _ _ |- _] => invert H
                |[H : App _ _ = If _ _ _ |- _] => invert H
+               |[H : If _ _ _ = Pair _ _ |- _] => invert H
+               |[H : App _ _ = Pair _ _ |- _] => invert H
+               |[H : Pair _ _ = If _ _ _ |- _] => invert H
+               |[H : Pair _ _ = App _ _ |- _] => invert H
              end.
 
 Lemma plug_step_uniq : forall C e e1 e2,
@@ -836,13 +837,21 @@ Proof.
   intros C e e1 e2 H H0.
   induction H; intros;
   try match goal with
-    |[H1: step_prim ?e _, H2: plug _ _ ?e |- _] =>
-     invert H1; invert H2; iauto; smash
+        |[H1: step_prim ?e _, H2: plug _ _ ?e |- _] =>
+         invert H1; invert H2; iauto; smash
+      end;
+  try match goal with
+    |[H: value (Pair ?e _), H1: plug _ _ ?e |- _] =>
+     invert H; eapply plug_values in H1; invert H1; iauto
+    |[H: value (Pair _ ?e), H1: plug _ _ ?e |- _] =>
+     invert H; eapply plug_values in H1; invert H1; iauto
   end;
   match goal with
     |[H: plug _ _ (App _ _) |- _] =>
      invert H; try solve [smash]
     |[H: plug _ _ (If _ _ _) |- _] =>
+     invert H; try solve [smash]
+    |[H: plug _ _ (Pair _ _) |- _] =>
      invert H; try solve [smash]
   end;
   match goal with
@@ -854,6 +863,12 @@ Proof.
      assert (C0 = C1 /\ P) by (eapply H; eauto); crush
     |[H: _ -> forall C _ _, _ -> _ -> ?C0 = C /\ _ |-
                       (CIf ?C0 _ _ = CIf ?C1 _ _ /\ ?P)] =>
+     assert (C0 = C1 /\ P) by (eapply H; eauto); crush
+    |[H: _ -> forall C _ _, _ -> _ -> ?C0 = C /\ _ |-
+       (CPair1 ?C0 ?e0 = CPair1 ?C1 ?e0 /\ ?P)] =>
+     assert (C0 = C1 /\ P) by (eapply H; eauto); crush
+    |[H: _ -> forall C _ _, _ -> _ -> ?C0 = C /\ _ |-
+       (CPair2 ?v0 ?C0 = CPair2 ?v0 ?C1 /\ ?P)] =>
      assert (C0 = C1 /\ P) by (eapply H; eauto); crush
   end.
 Qed.
@@ -1223,6 +1238,7 @@ Proof.
        end);
   match goal with
     |[H: (nil |-- (Abs _ _ _)) Bool |- _] => invert H
+    |[H: (nil |-- (Pair _ _)) Bool |- _] => invert H
   end.
 Qed.
 
@@ -1236,6 +1252,50 @@ Proof.
 Qed.
 
 Hint Resolve drop_fulfills.
+
+
+Lemma close_pair : forall Σ e1 e2,
+                    close Σ (Pair e1 e2) =
+                    Pair (close Σ e1) (close Σ e2).
+Proof.
+  intro Σ.
+  induction Σ; simpl; intuition.
+Qed.
+
+Hint Rewrite close_pair.
+
+
+Lemma TPair_compat : forall Γ Σ e1 e2 t1 t2,
+                      Γ |= Σ ->
+                      SN t1 (close Σ e1) ->
+                      SN t2 (close Σ e2) ->
+                      SN (Product t1 t2)
+                         (close Σ (Pair e1 e2)).
+Proof.
+  intros. crush;
+  repeat match goal with
+           |[H: SN _ _ |- _] =>
+            eapply sn_halts in H; invert H
+         end;
+  crush;
+  match goal with
+    |[H1: multi step ?e1 ?v1,
+          H2: multi step ?e2 ?v2 |-
+      halts (Pair ?e1 ?e2)] => eexists (Pair v1 v2)
+  end;
+  crush;
+  eapply multi_trans with (b := (Pair x0 (close Σ e2)));
+  match goal with
+    |[H: multi step ?e ?v |-
+      multi step (Pair ?e _) (Pair ?v _)] =>
+     eapply (multi_context H); iauto
+    |[H: multi step ?e ?v |-
+      multi step (Pair _ ?e) (Pair _ ?v)] =>
+     eapply (multi_context H); iauto
+  end.
+Qed.
+
+
 
 Theorem fundamental : forall e t Γ Σ,
                         Γ |-- e t ->
@@ -1257,4 +1317,6 @@ Proof.
   eapply TApp_compat; iauto.
 
   eapply TIf_compat; iauto.
+
+  eapply TPair_compat; iauto.
 Qed.
